coq proof for bank account

coq_inference/bank_account.v
@@ -8,35 +8,219 @@ Require Import chainmail.
 Require Import hoare.
 Require Import List.
 Require Import String.
+Require Import inference.
 Open Scope string_scope.
 Require Import CpdtTactics.
 Require Import Coq.Logic.FunctionalExtensionality.
 
 Module BankAccount(L : LanguageDef).
 
-  Import L.
-  Module L_Chainmail := Chainmail(L).
-  Import L_Chainmail.
-  Import L_Semantics.
+  Module L_Inference := Inference(L).
+  Import L_Inference.
   Open Scope reduce_scope.
   Open Scope chainmail_scope.
+  Open Scope hoare_scope.
+  Open Scope inference_scope.
 
   (** #<h2>#Variables#</h2>#*)
 
-  Definition src := n_ 0.
-  Definition amt := n_ 1.
-
   (** #<h2>#Account Class#</h2># *)
 
-  Definition Account := classID 1.
+  Definition Account := classID 100.
 
-  Definition deposit := methID 0.
+  Definition password := fieldID 101.
 
-  Parameter deposit_body : block.
+  Definition authenticate := methID 101.
+
+  Parameter authenticateBody : block.
+
+  Definition changePassword := methID 102.
+
+  Parameter changePasswordBody : block.
 
   Definition AccountDef := clazz Account
-                                 (update deposit deposit_body empty)
+                                 boundary
+                                 (⟦ password ↦ (t_cls Object) ⟧ empty)
+                                 (⟦ changePassword ↦ changePasswordBody ⟧
+                                    ⟦ authenticate ↦ authenticateBody  ⟧
+                                    empty)
                                  empty.
+
+  Definition pwd := (n_ 101).
+
+  (** #<h2>#Ledger Class#</h2># *)
+
+  Definition Ledger := classID 200.
+
+  Definition acc1 := fieldID 201.
+
+  Definition acc2 := fieldID 202.
+
+  Definition bal1 := fieldID 203.
+
+  Definition bal2 := fieldID 204.
+
+  Definition ledgerTransfer := methID 201.
+
+  Parameter ledgerTransferBody : block.
+
+  Definition ledgerGetBalance := gFieldID 201.
+
+  Definition acc := x_ (n_ 201).
+
+  Definition ledgerGetBalBody := e_if (e_eq (e_var acc) (e_acc_f (e_this) acc1))
+                                      (e_acc_f (e_this) acc1)
+                                      (e_if (e_eq (e_var acc) (e_acc_f (e_this) acc2))
+                                            (e_acc_f (e_this) bal2)
+                                      (e_int -1)).
+
+  Definition LedgerDef := clazz Ledger
+                                inside
+                                (⟦ bal2 ↦ t_int ⟧
+                                   ⟦ bal1 ↦ t_int ⟧
+                                   ⟦ acc2 ↦ (t_cls Account) ⟧
+                                   ⟦ acc1 ↦ (t_cls Account) ⟧
+                                   empty)
+                                (⟦ ledgerTransfer ↦ ledgerTransferBody ⟧ empty)
+                                (⟦ ledgerGetBalance ↦ (int, ledgerGetBalBody) ⟧empty).
+
+  Definition fromAcc := (n_ 202).
+
+  Definition toAcc := (n_ 203).
+
+  Definition amt := (n_ 204).
+
+  (** #<h2>#Bank Class#</h2># *)
+
+  Definition Bank := classID 300.
+
+  Definition book := fieldID 301.
+
+  Definition getBalance := gFieldID 302.
+
+  Definition getBalanceBody := (e_acc_g (e_acc_f (e_this) book) ledgerGetBalance (e_var acc)).
+
+  Definition transfer := methID 303.
+
+  Parameter transfer_body : block.
+
+  Definition BankDef := clazz Bank
+                              boundary
+                              (⟦ book ↦ (t_cls Ledger) ⟧ empty)
+                              (⟦ transfer ↦ transfer_body ⟧ empty)
+                              (⟦ getBalance ↦ (int, getBalanceBody) ⟧ empty).
+
+  (** #<h2>#Bank Module#</h2># *)
+
+  Definition BankMdl := (⟦ Account ↦ AccountDef ⟧
+                           ⟦ Ledger ↦ LedgerDef ⟧
+                           ⟦ Bank ↦ BankDef ⟧ empty).
+
+  (** #<h2>#Account Specifications#</h2># *)
+
+  Parameter authenticateBalanceChangeSpecification :
+    forall a a' b β bal, BankMdl ⊢ {pre: (a_class (e_ a) Account) ∧
+                                    (a_class (e_ a') Account) ∧
+                                    (a_class (e_ b)  Bank) ∧
+                                    (a_exp ((e_acc_g (e_ b) getBalance (e_ a')) ⩵ (e_int bal)))}
+                            m_call a authenticate β
+                            {post: a_exp ((e_acc_g (e_ b) getBalance (e_ a')) ⩵ (e_int bal))}.
+
+  Parameter changePasswordBalanceChangeSpecification :
+    forall a a' b β bal, BankMdl ⊢ {pre: (a_class (e_ a) Account) ∧
+                                    (a_class (e_ a') Account) ∧
+                                    (a_class (e_ b)  Bank) ∧
+                                    (a_exp ((e_acc_g (e_ b) getBalance (e_ a')) ⩵ (e_int bal)))}
+                            m_call a changePassword β
+                            {post: a_exp ((e_acc_g (e_ b) getBalance (e_ a')) ⩵ (e_int bal))}.
+
+  Lemma eq_implies_not_lt :
+    forall M e1 e2, M ⊢ (a_exp (e1 ⩵ e2)) ⊇ (¬ a_exp (e1 ⩻ e2)).
+    Admitted.
+
+  Lemma authBalChange :
+    forall a a' b bal ps,
+      BankMdl ⊢ ((a_class (e_ a') Account) ∧
+                 (a_class (e_ b) Bank) ∧
+                 (a_exp ((e_acc_g (e_ b) getBalance (e_ a')) ⩵ (e_int bal))) ∧
+                 (a_class (e_ a) Account) ∧
+                 (∃x.[ (a♢ 0) calls (a_ a) ◌ (am_ authenticate) ⟨ (fun v => Some (av_ v)) ∘ ps ⟩]))
+              to1 (a_exp ((e_acc_g (e_ b) getBalance (e_ a')) ⩻ (e_int bal)))
+              onlyIf (a_exp (e_false)).
+  Proof.
+    intros.
+    eapply if1_classical with (β := ps);
+      [|auto].
+    eapply hoare_consequence2; [|apply eq_implies_not_lt].
+    admit. (* add normal hoare logic rules *)
+
+  Admitted.
+
+  Lemma changePassowrdBalChange :
+    forall a a' b bal ps,
+      BankMdl ⊢ ((a_class (e_ a') Account) ∧
+                 (a_class (e_ b) Bank) ∧
+                 (a_exp ((e_acc_g (e_ b) getBalance (e_ a')) ⩵ (e_int bal))) ∧
+                 (a_class (e_ a) Account) ∧
+                 (∃x.[ (a♢ 0) calls (a_ a) ◌ (am_ changePassword) ⟨ (fun v => Some (av_ v)) ∘ ps ⟩]))
+              to1 (a_exp ((e_acc_g (e_ b) getBalance (e_ a')) ⩻ (e_int bal)))
+              onlyIf (a_exp (e_false)).
+  Proof.
+    intros.
+    apply if1_classical with (β := ps);
+      [|auto]. (* add simplification to tactic*)
+    eapply hoare_consequence2; [|apply eq_implies_not_lt].
+    admit. (* add normal hoare logic rules *)
+
+  Admitted.
+
+  Lemma ledgerTransferBalChange :
+    forall l a b bal ps v,
+      BankMdl ⊢ ((a_class (e_ l) Ledger) ∧
+                 (a_class (e_ a) Account) ∧
+                 (a_class (e_ b) Bank) ∧
+                 (a_exp ((e_acc_g (e_ b) getBalance (e_ a)) ⩵ (e_int bal))) ∧
+                 (a_exp ((e_acc_f (e_ a) password) ⩵ (e_val v))) ∧
+                (∃x.[ (a♢ 0) calls (a_ l) ◌ (am_ ledgerTransfer) ⟨ ps ⟩ ]))
+              to1 (a_exp ((e_acc_g (e_ b) getBalance (e_ a)) ⩻ (e_int bal)))
+              onlyIf (∃x.[∃x.[∃x.[ (a♢ 0) calls (a_ b) ◌ (am_ transfer) ⟨ ⟦ pwd ↦ (av_ v)⟧
+                                                                                ⟦ amt ↦ (a♢ 1)⟧
+                                                                                ⟦ fromAcc ↦ (a_ a) ⟧
+                                                                                ⟦ toAcc ↦ (a♢ 2) ⟧
+                                                                                empty ⟩]]]).
+  Proof.
+    intros.
+    eapply (if1_conseq);
+      [|apply conseq_refl
+       |apply conseq_refl
+       |apply absurd].
+    eapply (if1_conseq);
+      [|apply conseq_refl
+       |apply conseq_refl
+       |apply neg_false with (A:=wrapped(a_ l))].
+    
+  Admitted.
+
+  Lemma bankTransferBalChange :
+    forall l a b b' bal ps v,
+      BankMdl ⊢ ((a_class (e_ l) Ledger) ∧
+                 (a_class (e_ a) Account) ∧
+                 (a_class (e_ b) Bank) ∧
+                 (a_class (e_ b') Bank) ∧
+                 (a_exp ((e_acc_g (e_ b) getBalance (e_ a)) ⩵ (e_int bal))) ∧
+                 (a_exp ((e_acc_f (e_ a) password) ⩵ (e_val v))) ∧
+                (∃x.[ (a♢ 0) calls (a_ b) ◌ (am_ transfer) ⟨ ps ⟩ ]))
+              to1 (a_exp ((e_acc_g (e_ b) getBalance (e_ a)) ⩻ (e_int bal)))
+              onlyIf (∃x.[∃x.[∃x.[ (a♢ 0) calls (a_ b) ◌ (am_ transfer) ⟨ ⟦ pwd ↦ (av_ v)⟧
+                                                                                ⟦ amt ↦ (a♢ 1)⟧
+                                                                                ⟦ fromAcc ↦ (a_ a) ⟧
+                                                                                ⟦ toAcc ↦ (a♢ 2) ⟧
+                                                                                empty ⟩]]]).
+  Proof.
+    intros.
+    
+  Admitted.
+
 
   Close Scope chainmail_scope.
   Close Scope reduce_scope.
