coq_inference/inference.v
@@ -6,21 +6,26 @@ Require Import defs.
 Require Import operational_semantics.
 Require Import List.
 Require Import chainmail.
+Require Import hoare.
 
 Module Inference(L : LanguageDef).
 
-  Import L.
+  Export L.
   Module L_Semantics := AbstractOperationalSemantics(L).
-  Import L_Semantics.
-  Module L_Chainmail := Chainmail(L).
-  Import L_Chainmail.
+  Export L_Semantics.
+  Module L_Hoare := Hoare(L).
+  Export L_Hoare.
+  (*)Module L_Chainmail := Chainmail(L).
+  Import L_Chainmail.*)
+
+  Open Scope chainmail_scope.
+  Open Scope reduce_scope.
+  Open Scope hoare_scope.
+  Declare Scope inference_scope.
 
   Reserved Notation "M '⊢' A1 'to' A2 'onlyIf' A3" (at level 40).
   Reserved Notation "M '⊢' A1 'to' A2 'onlyThrough' A3" (at level 40).
   Reserved Notation "M '⊢' A1 'to1' A2 'onlyIf' A3" (at level 40).
-
-  Open Scope chainmail_scope.
-  Open Scope reduce_scope.
 
   Lemma caller_ext :
     forall M α1 α2 m β, M ⊢ α1 calls α2 ◌ m ⟨ β ⟩ ⊇ α1 external.
@@ -44,9 +49,59 @@ Module Inference(L : LanguageDef).
 
   Lemma fld_type :
     forall M e C CDef f D, ⟦ C ↦ CDef ⟧_∈ M ->
-                      ⟦ f ↦ D ⟧_∈ c_fields CDef ->
+                      ⟦ f ↦ (t_cls D) ⟧_∈ c_fields CDef ->
                       M ⊢ a_class e C ⊇ a_class ((e_acc_f e f)) D.
   Admitted.
+
+  Lemma absurd :
+    forall M A, M ⊢ (a_exp (e_false)) ⊇ A.
+  Admitted.
+
+  Lemma conseq_refl :
+    forall M A, M ⊢ A ⊇ A.
+  Admitted.
+
+  Lemma neg_false :
+    forall M A, M ⊢ (A ∧ ¬ A) ⊇ (a_exp (e_false)).
+  Admitted.
+
+  Inductive intrnl : mdl -> asrt -> exp -> Prop :=
+  | i_int : forall M A i, intrnl M A (e_int i)
+  | i_true : forall M A, intrnl M A (e_true)
+  | i_false : forall M A, intrnl M A (e_false)
+  | i_null : forall M A, intrnl M A (e_null)
+  | i_obj : forall M A α C, M ⊢ A ⊇ (a_class (e_addr α) C) ->
+                       C ∈ M ->
+                       intrnl M A (e_addr α)
+  | i_var : forall M A x C, M ⊢ A ⊇ (a_class (e_var x) C) ->
+                       C ∈ M ->
+                       intrnl M A (e_var x)
+  | i_fld : forall M A e C CDef f D, intrnl M A e ->
+                                M ⊢ A ⊇ (a_class e C) ->
+                                ⟦ C ↦ CDef ⟧_∈ M ->
+                                ⟦ f ↦ (t_cls D) ⟧_∈ c_fields CDef ->
+                                D ∈ M ->
+                                intrnl M A (e_acc_f e f)
+  | i_ghost : forall M A e1 e2 C CDef e g, intrnl M A e1 ->
+                                      intrnl M A e2 ->
+                                      M ⊢ A ⊇ (a_class e1 C) ->
+                                      ⟦ C ↦ CDef ⟧_∈ M ->
+                                      ⟦ g ↦ (int, e) ⟧_∈ c_g_fields CDef ->
+                                      intrnl M A (e_acc_g e1 g e2).
+
+  Inductive enc : mdl -> asrt -> asrt -> Prop :=
+  | enc_intrnl : forall M A e, intrnl M A e ->
+                          enc M A (a_exp e)
+  | enc_field : forall M A e f, intrnl M A e ->
+                           enc M A (a_exp (e_acc_f e f))
+  | enc_int_acc : forall M A α1 α2, M ⊢ A ⊇ (α1 internal) ->
+                               enc M A (α1 access α2)
+  | enc_wrapped1 : forall M A α, enc M A (wrapped α)
+  | enc_wrapped2 : forall M A α1 α2, M ⊢ A ⊇ (wrapped α2) ->
+                                enc M A (¬ α1 access α2)
+  | enc_conseq : forall M A1 A2 A, M ⊢ A1 ⊇ A2 ->
+                              enc M A2 A ->
+                              enc M A1 A.
 
   Inductive only_if : mdl -> asrt -> asrt -> asrt -> Prop :=
   | if_start  : forall M A1 A2, M ⊢ A1 to A2 onlyIf A1
@@ -108,6 +163,19 @@ Module Inference(L : LanguageDef).
   "M '⊢' A1 'to' A2 'onlyThrough' A3" := (only_through M A1 A2 A3)
 
   with only_if1 : mdl -> asrt -> asrt -> asrt -> Prop :=
+  | if1_classical : forall M P1 α C m β β' P2 P,
+      M ⊢ {pre: ((a_class (e_addr α) C) ∧ P1 ∧ ¬ P) } (m_call α m β) {post: ¬ P2} ->
+      β' = (fun v => Some (av_ v)) ∘ β  ->
+      M ⊢ (P1 ∧ (a_class (e_addr α) C) ∧ (∃x.[ (a♢ 0) calls (a_ α) ◌ (am_ m) ⟨ β' ⟩])) to1 P2 onlyIf P
+  | if1_wrapped : forall M α C P m β α',
+      M ⊢ {pre: (a_class (e_addr α) C) ∧ ¬ P } (m_call α m β) {post: a_exp ((e♢ 0) ⩵̸ (e_ α'))} ->
+      M ⊢ (wrapped (a_ α') ∧ (a_class (e_ α) C) ∧ (∃x.[ (a♢ 0) calls (a_ α) ◌ (am_ m) ⟨ (fun v => Some (av_ v)) ∘ β ⟩ ]))
+        to1 (¬ (wrapped (a_ α'))) onlyIf P
+  | if1_internal : forall M A1 A2 A3,
+      (forall C CDef m α β, ⟦ C ↦ CDef ⟧_∈ M ->
+                       m ∈ c_meths CDef ->
+      M ⊢ (A1 ∧ (a_class (e_ α) C) ∧ ∃x.[ (a♢ 0) calls (a_ α) ◌ (am_ m) ⟨ β ⟩]) to1 A2 onlyIf A3) ->
+      M ⊢ A1 to1 A2 onlyIf A3
   | if1_if : forall M A1 A2 A3, M ⊢ A1 to A2 onlyIf A3 ->
                            M ⊢ A1 to1 A2 onlyIf A3
   | if1_conseq : forall M A1 A1' A2 A2' A A', M ⊢ A1' to1 A2' onlyIf A' ->
@@ -128,6 +196,8 @@ Module Inference(L : LanguageDef).
   where
   "M '⊢' A1 'to1' A2 'onlyIf' A3" := (only_if1 M A1 A2 A3).
 
-
+  Close Scope inference_scope.
+  Close Scope chainmail_scope.
+  Close Scope reduce_scope.
 
 End Inference.
